work on cache state machine

concurrency/scache/CacheSM.i.dfy
@@ -1,40 +1,103 @@
 include "../framework/DiskSSM.s.dfy"
 include "CacheSpec.s.dfy"
+include "../../lib/Base/Option.s.dfy"
 
 module CacheSSM refines DiskSSM(CacheIfc) {
+  import opened Options
+
   datatype Status = Empty | Reading | Clean | Dirty | Writeback
 
-  datatype CacheEntry = CacheEntry(
-    disk_idx: int, // meaningless if Status == Empty
-    cache_idx: int,
-    data: seq<byte>
+  datatype Entry = Entry(
+    disk_idx: nat, // meaningless if Status == Empty
+    data: seq<byte> // meaningless if Status in {Empty, Reading}
   )
 
   datatype M = M(
-    disk_idx_to_cache_idx: map<nat, nat>,
-    entries: map<nat, CacheEntry>,
-    statuses: map<nat, Status>
-    disk_write_reqs: map<nat, seq<byte>>,
-    disk_write_resps: set<nat>,
-    disk_read_reqs: set<nat>,
-    disk_read_resp: map<nat, seq<byte>>,
+    disk_idx_to_cache_idx: map<nat, Option<nat>>,
+    entries: map<nat, Entry>,
+    statuses: map<nat, Status>,
+    write_reqs: map<nat, seq<byte>>,
+    write_resps: set<nat>,
+    read_reqs: set<nat>,
+    read_resps: map<nat, seq<byte>>,
+    tickets: map<RequestId, IOIfc.Input>,
+    stubs: map<RequestId, IOIfc.Output>
   ) | Fail
 
+  function union_map<K, V>(m1: map<K, V>, m2: map<K, V>) : map<K, V> {
+    map k | k in m1.Keys + m2.Keys :: if k in m1 then m1[k] else m2[k]
+  }
+
   function dot(x: M, y: M) : M {
-    if x.M? && y.M? &&
-        && disjoint_maps(x.disk_idx_to_cache_idx, y.disk_idx_to_cache_idx)
-        && disjoint_maps(x.entries, y.entries)
-        && disjoint_maps(x.statuses, y.statuses)
+    if x.M? && y.M?
+        && x.disk_idx_to_cache_idx.Keys !! y.disk_idx_to_cache_idx.Keys
+        && x.entries.Keys !! y.entries.Keys
+        && x.statuses.Keys !! y.statuses.Keys
+        && x.write_reqs.Keys !! y.write_reqs.Keys
+        && x.write_resps !! y.write_resps
+        && x.read_reqs !! y.read_reqs
+        && x.read_resps.Keys !! y.read_resps.Keys
+        && x.tickets.Keys !! y.tickets.Keys
+        && x.stubs.Keys !! y.stubs.Keys
     then
       M(
         union_map(x.disk_idx_to_cache_idx, y.disk_idx_to_cache_idx),
         union_map(x.entries, y.entries),
-        union_map(x.statuses, y.statuses)
+        union_map(x.statuses, y.statuses),
+        union_map(x.write_reqs, y.write_reqs),
+        x.write_resps + y.write_resps,
+        x.read_reqs + y.read_reqs,
+        union_map(x.read_resps, y.read_resps),
+        union_map(x.tickets, y.tickets),
+        union_map(x.stubs, y.stubs)
       )
+    else
+      Fail
+  }
+
+  function DiskIdxToCacheIdx(disk_idx: nat, cache_idx: Option<nat>) : M {
+    M(map[disk_idx := cache_idx],
+      map[], map[], map[], {}, {}, map[], map[], map[])
+  }
+
+  function CacheEntry(cache_idx: nat, disk_idx: nat, data: seq<byte>) : M {
+    M(map[],
+      map[cache_idx := Entry(disk_idx, data)],
+      map[], map[], {}, {}, map[], map[], map[])
+  }
+
+  function CacheStatus(cache_idx: nat, status: Status) : M {
+    M(map[], map[],
+      map[cache_idx := status],
+      map[], {}, {}, map[], map[], map[])
+  }
+
+  function WriteReq(disk_idx: nat, data: seq<byte>) : M {
+    M(map[], map[], map[],
+      map[disk_idx := data],
+      {}, {}, map[], map[], map[])
+  }
+
+  function WriteResp(disk_idx: nat) : M {
+    M(map[], map[], map[], map[],
+      {disk_idx},
+      {}, map[], map[], map[])
+  }
+
+  function ReadReq(disk_idx: nat) : M {
+    M(map[], map[], map[], map[], {},
+      {disk_idx},
+      map[], map[], map[])
+  }
+
+  function ReadResp(disk_idx: nat, data: seq<byte>) : M {
+    M(map[], map[], map[], map[], {}, {},
+      map[disk_idx := data],
+      map[], map[])
   }
 
   function unit() : M {
-    M(map[], map[], map[])
+    M(map[], map[], map[], map[], {}, {}, map[], map[], map[])
   }
 
   function Ticket(rid: RequestId, input: IOIfc.Input) : M
@@ -43,28 +106,102 @@ module CacheSSM refines DiskSSM(CacheIfc) {
   // By returning a set of request ids "in use", we enforce that
   // there are only a finite number of them (i.e., it is always possible to find
   // a free one).
-  function request_ids_in_use(m: M) : set<RequestId>
+  function request_ids_in_use(m: M) : set<RequestId> {
+    if m.M? then
+      m.tickets.Keys + m.stubs.Keys
+    else
+      {}
+  }
 
-  function DiskWriteReq(disk_addr: int, data: seq<byte>) : M
-  function DiskWriteResp(disk_addr: int, len: int) : M
+  function DiskWriteReq(disk_addr: nat, data: seq<byte>) : M
+  function DiskWriteResp(disk_addr: nat, len: nat) : M
 
-  function DiskReadReq(disk_addr: int, len: int) : M
-  function DiskReadResp(disk_addr: int, data: seq<byte>) : M
+  function DiskReadReq(disk_addr: nat, len: nat) : M
+  function DiskReadResp(disk_addr: nat, data: seq<byte>) : M
 
   predicate Init(s: M)
+
+  function dot3(a: M, b: M, c: M) : M {
+    dot(dot(a, b), c)
+  }
+
+  function dot4(a: M, b: M, c: M, d: M) : M {
+    dot(dot(dot(a, b), c), d)
+  }
+
+  predicate StartRead(shard: M, shard': M,
+      cache_idx: nat, disk_idx: nat, junk_data: seq<byte>, junk_disk_idx: nat) {
+    && shard == dot3(
+        CacheStatus(cache_idx, Empty),
+        CacheEntry(cache_idx, junk_disk_idx, junk_data),
+        DiskIdxToCacheIdx(disk_idx, None)
+       )
+    && shard' == dot4(
+        CacheStatus(cache_idx, Reading),
+        CacheEntry(cache_idx, disk_idx, junk_data),
+        DiskIdxToCacheIdx(disk_idx, Some(cache_idx)),
+        ReadReq(disk_idx)
+       )
+  }
+
+  predicate FinishRead(shard: M, shard': M,
+      cache_idx: nat, disk_idx: nat, junk_data: seq<byte>, data: seq<byte>,
+      status: Status) {
+    && shard == dot3(
+        CacheStatus(cache_idx, status),
+        CacheEntry(cache_idx, disk_idx, junk_data),
+        ReadResp(disk_idx, data)
+       )
+    && shard' == dot(
+        CacheStatus(cache_idx, Clean),
+        CacheEntry(cache_idx, disk_idx, data)
+       )
+  }
+
+  predicate StartWriteback(shard: M, shard': M,
+      cache_idx: nat, disk_idx: nat, data: seq<byte>) {
+    && shard == dot(
+        CacheStatus(cache_idx, Dirty),
+        CacheEntry(cache_idx, disk_idx, data)
+       )
+    && shard' == dot3(
+        CacheStatus(cache_idx, Writeback),
+        CacheEntry(cache_idx, disk_idx, data),
+        WriteReq(disk_idx, data)
+       )
+  }
+
+  predicate FinishWriteback(shard: M, shard': M,
+      cache_idx: nat, disk_idx: nat, data: seq<byte>, status: Status) {
+    && shard == dot(
+        CacheStatus(cache_idx, status),
+        WriteResp(disk_idx)
+       )
+    && shard' == 
+        CacheStatus(cache_idx, Clean)
+  }
+
+  predicate Evict(shard: M, shard': M,
+      cache_idx: nat, disk_idx: nat, data: seq<byte>, cache_idx2: Option<nat>) {
+    && shard == dot3(
+        CacheStatus(cache_idx, Clean),
+        CacheEntry(cache_idx, disk_idx, data),
+        DiskIdxToCacheIdx(disk_idx, cache_idx2)
+      )
+    && shard == dot3(
+        CacheStatus(cache_idx, Empty),
+        CacheEntry(cache_idx, disk_idx, data),
+        DiskIdxToCacheIdx(disk_idx, None)
+      )
+  }
+
   predicate Internal(shard: M, shard': M)
 
-  predicate NewTicket(whole: M, whole': M, rid: RequestId, input: IOIfc.Input) {
-    && rid !in request_ids_in_use(whole)
-    && whole' == dot(whole, Ticket(rid, input))
+  predicate Inv(s: M) {
+    true
   }
 
-  predicate ConsumeStub(whole: M, whole': M, rid: RequestId, output: IOIfc.Output) {
-    && whole == dot(whole', Stub(rid, output))
-  }
-
-  predicate Inv(s: M)
-
+/*
   lemma InitImpliesInv(s: M)
   requires Init(s)
   ensures Inv(s)
@@ -84,11 +221,11 @@ module CacheSSM refines DiskSSM(CacheIfc) {
   requires ConsumeStub(whole, whole', rid, output)
   ensures Inv(whole')
 
-  lemma ProcessReadPreservesInv(disk_addr: int, data: seq<byte>, rest: M)
+  lemma ProcessReadPreservesInv(disk_addr: nat, data: seq<byte>, rest: M)
   requires Inv(dot(DiskReadReq(disk_addr, |data|), rest))
   ensures Inv(dot(DiskReadResp(disk_addr, data), rest))
 
-  lemma ProcessWritePreservesInv(disk_addr: int, data: seq<byte>, rest: M)
+  lemma ProcessWritePreservesInv(disk_addr: nat, data: seq<byte>, rest: M)
   requires Inv(dot(DiskWriteReq(disk_addr, data), rest))
   ensures Inv(dot(DiskWriteResp(disk_addr, |data|), rest))
 
@@ -105,4 +242,5 @@ module CacheSSM refines DiskSSM(CacheIfc) {
   returns (s: M)
   ensures Inv(s)
 
+*/
 }
